Structure...

LogicalRefinement/Denot/Basic.lean
@@ -4,3 +4,191 @@ import LogicalRefinement.Stlc
 
 open AnnotSort
 open Annot
+
+--TODO: should this be an inductive type?
+def Term.denote_ty (A: Term) 
+  {Γ: Stlc.Context}
+  (σ: Sparsity)
+  (G: Γ.interp)
+  (a: A.stlc_ty.interp): Prop
+  := match A with
+  | const TermKind.unit => 
+    match a with
+    | some () => True
+    | none => False
+  | abs TermKind.pi A B => 
+    match a with
+    | some a =>
+      ∀x: A.stlc_ty.interp,
+        A.denote_ty σ G x ->
+        @denote_ty B (A.stlc_ty::Γ) (true::σ) (x, G) (x.bind_val a)
+    | none => False
+  | abs TermKind.sigma A B => 
+    match a with
+    | some (a, b) => 
+      let a := Ty.eager a;
+      let b := Ty.eager b;
+      A.denote_ty σ G a ∧ @denote_ty B (A.stlc_ty::Γ) (true::σ) (a, G) b
+    | none => False
+  | bin TermKind.coprod A B =>
+    match a with
+    | some a => 
+      match a with
+      | Sum.inl a => A.denote_ty σ G (Ty.eager a)
+      | Sum.inr b => B.denote_ty σ G (Ty.eager b)
+    | none => False
+  | abs TermKind.assume φ A => 
+    a ≠ none ∧
+    ((φ.denote_ty σ G none) -> (A.denote_ty (false::σ) G a))
+  | abs TermKind.set A φ => 
+    A.denote_ty σ G a ∧ @denote_ty φ (A.stlc_ty::Γ) (true::σ) (a, G) none
+  | abs TermKind.intersect A B => 
+    a ≠ none ∧
+    ∀x: A.stlc_ty.interp,
+      A.denote_ty σ G x ->
+      @denote_ty B (A.stlc_ty::Γ) (true::σ) (x, G) a
+  | abs TermKind.union A B => 
+    a ≠ none ∧
+    ∃x: A.stlc_ty.interp,
+      A.denote_ty σ G x ∧
+      @denote_ty B (A.stlc_ty::Γ) (true::σ) (x, G) a
+  | const TermKind.top => True
+  | const TermKind.bot => False
+  | abs TermKind.dimplies A B => 
+    --TODO: think about this...
+    (A.denote_ty σ G none) -> (B.denote_ty (false::σ) G none)
+  | abs TermKind.dand A B =>
+    --TODO: think about this...
+    A.denote_ty σ G none ∧ B.denote_ty (false::σ) G none
+  | bin TermKind.or A B => 
+    A.denote_ty σ G none ∨ B.denote_ty σ G none
+  | abs TermKind.forall_ A φ => 
+    ∀x: A.stlc_ty.interp,
+      A.denote_ty σ G x ->
+      @denote_ty φ (A.stlc_ty::Γ) (true::σ) (x, G) none
+  | abs TermKind.exists_ A φ => 
+    ∃x: A.stlc_ty.interp,
+      A.denote_ty σ G x ∧
+      @denote_ty φ (A.stlc_ty::Γ) (true::σ) (x, G) none
+  | tri TermKind.eq A x y => 
+    ∃ px: Γ ⊧ x.stlc σ: A.stlc_ty, 
+    ∃ py: Γ ⊧ y.stlc σ: A.stlc_ty,
+    px.interp G = py.interp G
+  | const TermKind.nats => 
+    match a with
+    | some _ => True
+    | none => False
+  | _ => False
+
+abbrev Term.denote_prop (A: Term) 
+  {Γ: Stlc.Context}
+  (σ: Sparsity)
+  (G: Γ.interp): Prop
+  := A.denote_ty σ G none
+
+abbrev Term.denote_ty' (A: Term) {Γ: Context}
+  (G: Γ.upgrade.stlc.interp)
+  (a: A.stlc_ty.interp): Prop
+  := A.denote_ty Γ.upgrade.sparsity G a
+
+abbrev Term.denote_prop' (A: Term) {Γ: Context}
+  (G: Γ.upgrade.stlc.interp): Prop
+  := A.denote_prop Γ.upgrade.sparsity G
+
+notation G "⊧" a "↓" σ "∈" A => Term.denote_ty A σ G a
+notation G "⊧" a "∈" A => Term.denote_ty' A G a
+
+theorem Term.denote_ty_transport 
+  {A: Term} {Γ G} {a: A.stlc_ty.interp}
+  {A' Γ' G' a'}
+  (HA: A = A')
+  (HΓ: Γ = Γ')
+  (HG: G = HΓ ▸ G')
+  (Ha: a' = HA ▸ a)
+  : @denote_ty' A Γ G a -> @denote_ty' A' Γ' G' a'
+  := by {
+    cases HA;
+    cases HΓ;
+    cases HG;
+    cases Ha;
+    exact id
+  }
+
+theorem HasType.denote_ty_non_null {Δ: Stlc.Context} {G: Δ.interp}:
+  (Γ ⊢ A: type) ->
+  ¬(A.denote_ty σ G none)
+  := by {
+    generalize HS: sort type = S;
+    intro HA;
+    induction HA with
+    | set _ _ IA Iφ => 
+      dsimp only [Term.denote_ty]
+      intro ⟨HA, Hφ⟩;
+      exact IA rfl HA
+    | assume _ _ Iφ IA => 
+      intro ⟨H, _⟩;
+      exact H rfl
+    | intersect => 
+      intro ⟨H, _⟩;
+      exact H rfl
+    | union => 
+      intro ⟨H, _⟩;
+      exact H rfl
+    | _ => cases HS <;> intro H <;> cases H
+  }
+  
+theorem HasType.denote_ty_some {Δ: Stlc.Context} {G: Δ.interp}
+  (H: Γ ⊢ A: type)
+  (D: A.denote_ty σ G a)
+  : ∃a': A.stlc_ty.interp_val, a = some a'
+  := match a with
+    | some a => ⟨a, rfl⟩
+    | none => False.elim (H.denote_ty_non_null D)
+
+theorem interp_eq_none
+  : @Eq.rec Ty a (λx _ => Ty.interp x) none x p = none := by {
+    cases p <;> rfl
+  }
+
+theorem interp_eq_none' {n: Ty.interp a}
+  : n = none -> @Eq.rec Ty a (λx _ => Ty.interp x) n x p = none := by {
+    intro H;
+    cases H <;>
+    cases p <;> rfl
+  }
+
+theorem interp_eq_some
+  : @Eq.rec Ty a (λx _ => Ty.interp x) (some v) x p = (some (p ▸ v)) := by {
+    cases p <;> rfl
+  }
+
+abbrev Annot.denote (A: Annot) {Γ: Stlc.Context}
+  (σ: Sparsity)
+  (G: Γ.interp)
+  (a: A.stlc_ty.interp): Prop
+  := match A with
+  | sort s => True
+  | expr type A => A.denote_ty σ G a
+  | expr prop A => A.denote_ty σ G none
+
+abbrev Annot.denote' (A: Annot) (Γ: Context)
+  (G: Γ.upgrade.stlc.interp)
+  (a: A.stlc_ty.interp): Prop
+  := match A with
+  | sort s => True
+  | expr type A => A.denote_ty' G a
+  | expr prop A => A.denote_ty' G none
+
+notation G "⊧" a "↓" σ "∈:" A => Annot.denote A σ G a
+notation G "⊧" a "∈:" A => Annot.denote' A G a
+
+def Context.denote: (Γ: Context) -> Γ.upgrade.stlc.interp -> Prop
+| [], () => True
+| (Hyp.mk A (HypKind.val type))::Γ, (a, G) => 
+  A.denote_ty (upgrade Γ).sparsity G a ∧ denote Γ G
+| (Hyp.mk φ (HypKind.val prop))::Γ, G =>
+  φ.denote_ty (upgrade Γ).sparsity G none ∧ denote Γ G
+| (Hyp.mk A HypKind.gst)::Γ, (a, G) =>
+  A.denote_ty (upgrade Γ).sparsity G a ∧ denote Γ G
+
+notation G "⊧" "✓" Γ => Context.denote Γ G
