LogicalRefinement/Denot/Regular.lean
@@ -1,0 +1,410 @@
+import LogicalRefinement.Untyped
+import LogicalRefinement.Typed
+import LogicalRefinement.Stlc
+import LogicalRefinement.Denot.Basic
+import LogicalRefinement.Denot.Wk
+import LogicalRefinement.Denot.Subst
+
+open AnnotSort
+open Annot
+
+
+theorem HasVar.denote_annot
+  (Hv: HasVar Γ n (HypKind.val s) A)
+  (HΓ: IsCtx Γ)
+  (G: Γ.upgrade.stlc.interp)
+  (HG: G ⊧ ✓Γ)
+  : (expr s A).denote' Γ G ((HΓ.var Hv).stlc.interp G.downgrade)
+  := by {
+    induction Γ generalizing s n A with
+    | nil => cases Hv
+    | cons H Γ I =>   
+      cases H with
+      | mk A k =>
+        cases k with
+        | val s => 
+          cases s with
+          | type => 
+            let (x, G) := G;
+            have ⟨Hx, HG⟩ := HG;
+            cases Hv with
+            | zero Hk => 
+              cases Hk;
+              simp only [denote, Context.stlc]
+              apply Term.denote_wk1_ty _ _ Γ x G _ _ _ Hx
+              rw [Stlc.Context.interp.downgrade_ty]
+              rw [Stlc.HasType.interp_var]
+              dsimp only [Stlc.HasVar.interp, Sparsity.ix]
+              simp only [Eq.mp, Eq.mpr]
+              conv =>
+                rhs
+                rw [monorecursor]
+                skip
+                rw [<-A.stlc_ty_wk1]
+            | succ Hv => 
+              cases HΓ with
+              | cons_val HΓ =>
+                have I' := I Hv HΓ G HG;
+                cases s with
+                | type =>
+                  simp only [denote, Context.stlc]
+                  apply Term.denote_wk1_ty _ _ Γ x G _ _ _ I'
+                  rw [monorecursor]
+                  rename Nat => n;
+                  rw [Stlc.HasType.interp_transport_mono]
+                  rw [Stlc.Context.interp.downgrade_ty]
+                  rw [Stlc.HasType.var_interp_wk1]
+                  rfl
+                  rw [Term.stlc_var]
+                  dsimp only [Sparsity.stlc]
+                  split
+                  . rfl
+                  . have s := Hv.sigma_ty;
+                    contradiction
+                  rw [Term.stlc_ty_wk1]
+                  constructor
+                  exact Hv.stlc
+                  rw [Term.stlc_var]
+                  dsimp only [Sparsity.stlc]
+                  split
+                  . rfl
+                  . have s := Hv.sigma_ty;
+                    contradiction
+                  rw [Term.stlc_ty_wk1]
+                  rfl
+                  rw [Term.stlc_ty_wk1]
+                  rfl
+                | prop => 
+                  simp only [denote]
+                  exact 
+                    Term.denote_wk1_ty _ _ Γ x G 
+                      none none (by rw [interp_eq_none]) I';
+          | prop => 
+            have ⟨Hx, HG⟩ := HG;
+            cases Hv with
+            | zero Hk => 
+              cases Hk;
+              simp only [denote, Context.stlc]
+              apply Term.denote_wk1_prop _ _ Γ G _ _ _ Hx
+              rw [interp_eq_none]
+            | succ Hv => 
+              cases HΓ with
+              | cons_val HΓ =>
+                have I' := I Hv HΓ G HG;
+                cases s with
+                | type =>                   
+                  simp only [denote, Context.stlc]
+                  apply Term.denote_wk1_prop _ _ Γ G _ _ _ I'
+                  rw [monorecursor]
+                  rename Nat => n;
+                  rw [Stlc.HasType.interp_transport_mono]
+                  rfl
+                  rw [Term.stlc_var]
+                  dsimp only [Sparsity.stlc]
+                  split
+                  . dsimp only [Term.stlc, Sparsity.stlc]
+                    split
+                    . rfl
+                    . have s := Hv.sigma_ty;
+                      contradiction
+                  . have s := Hv.sigma_ty;
+                    contradiction
+                  rw [Term.stlc_ty_wk1]
+                  constructor
+                  rw [Term.stlc_ty_wk1]
+                  rfl
+                | prop => 
+                  simp only [denote]
+                  exact 
+                    Term.denote_wk1_prop _ _ Γ G 
+                      none none (by rw [interp_eq_none]) I';
+        | gst => 
+          cases Hv with
+          | zero Hk => cases Hk
+          | succ Hv => 
+            cases HΓ with
+            | cons_gst HΓ => 
+              let (x, G) := G;
+              have ⟨Hx, HG⟩ := HG;
+              have I' := I Hv HΓ G HG;
+              cases s with
+              | type => 
+                simp only [denote, Context.stlc]
+                apply Term.denote_wk1_gst _ _ Γ x G _ _ _ I'
+                rw [monorecursor]
+                rw [Stlc.HasType.interp_transport_mono]
+                rw [Stlc.Context.interp.downgrade_gst]
+                rfl
+                rw [Term.stlc_ty_wk1]
+                rfl
+                rw [Term.stlc_ty_wk1]
+                rfl
+              | prop => 
+                simp only [denote]
+                exact 
+                  Term.denote_wk1_gst _ _ Γ x G 
+                    none none (by rw [interp_eq_none]) I';
+  }
+
+theorem HasType.sym_axiom {Γ A} (HA: Γ ⊢ A: type):
+  ∀{G: Γ.upgrade.stlc.interp}, (Term.sym_ty A).denote_prop' G
+  := by {
+    intro G;
+    dsimp only [
+      Term.denote_prop', 
+      Term.denote_prop,
+      Term.denote_ty,
+      Term.sym_ty, Term.sym_ty_tmp, Term.subst0, Term.subst,
+      Subst.lift, Subst.wk1, Term.wk1, Term.to_subst,
+      Wk.var, Term.wk
+    ]
+    intro x Hx y Hy ⟨px, py, Hxy⟩;
+    sorry
+  }
+
+theorem HasType.trans_axiom {Γ A} (HA: Γ ⊢ A: type):
+  ∀{G: Γ.upgrade.stlc.interp}, (Term.trans_ty A).denote_prop' G
+  := by {
+    intro G;
+    dsimp only [
+      Term.denote_prop', 
+      Term.denote_prop,
+      Term.denote_ty,
+      Term.sym_ty, Term.sym_ty_tmp, Term.subst0, Term.subst,
+      Subst.lift, Subst.wk1, Term.wk1, Term.to_subst,
+      Wk.var, Term.wk
+    ]
+    intro x Hx y Hy z Hz ⟨px, py, Hxy⟩ ⟨py, pz, Hyz⟩;
+    sorry
+  }
+
+theorem HasType.denote
+  (H: Γ ⊢ a: A)
+  (HΓ: IsCtx Γ)
+  (G: Γ.upgrade.stlc.interp)
+  (HG: Γ.denote G)
+  : A.denote' Γ G (H.stlc.interp G.downgrade)
+  := by {
+    --TODO: replace with a recursive match?
+    induction H with
+    | var HA Hv IA => exact Hv.denote_annot HΓ G HG
+    | lam Hs HA Is IA => 
+      stop
+      intro x Hx
+      cases x with
+      | some x => 
+        --TODO: make this a simp attribute mmkay...
+        dsimp only [
+          Annot.stlc_ty, term, Term.stlc_ty, Term.stlc, 
+          Stlc.HasType.interp, 
+          Ty.interp.app, Ty.interp.bind_val
+        ]
+        rw [<-Stlc.Context.interp.downgrade_ty]
+        apply Is
+        constructor
+        exact HΓ
+        exact HA
+        exact ⟨Hx, HG⟩
+      | none => exact False.elim (HA.denote_ty_non_null Hx)
+    | @app Γ A B l r HAB Hl Hr IA Il Ir => 
+      stop
+      dsimp only [Annot.denote]
+      dsimp only [
+        Annot.stlc_ty, term, Term.stlc_ty, Term.stlc, 
+        Stlc.HasType.interp, 
+        Ty.interp.app
+      ]
+      generalize Hlg:
+        Stlc.HasType.interp
+        (_ : _⊧Term.stlc l _:_)
+        (Stlc.Context.interp.downgrade G) = li;
+      have Il' := Hlg ▸ (Il HΓ G HG);
+      generalize Hrg:
+        Stlc.HasType.interp
+        (_ : _⊧Term.stlc r _:_)
+        (Stlc.Context.interp.downgrade G) = ri;
+      have Ir' := Hrg ▸ (Ir HΓ G HG);
+      have HA: Γ ⊢ A: type := by cases HAB; assumption;
+      have HB: ((Hyp.val A type)::Γ) ⊢ B: type := by cases HAB; assumption;
+      cases li with
+      | some li => 
+        cases ri with
+        | some ri => 
+          have Ilr := Il' (some ri) Ir';
+          simp only []
+          dsimp only [Annot.denote, Term.denote_ty, denote', Term.denote_ty'] at Il'
+          dsimp only [Annot.denote, Term.denote_ty, denote']
+          apply HasType.denote_subst0' Hr HB.stlc_ty_subst.symm _ Hrg.symm Ilr
+          rw [monorecursor]
+          rfl
+        | none => exact False.elim (HA.denote_ty_non_null Ir')
+      | none => exact False.elim (HAB.denote_ty_non_null Il')
+    | @pair Γ A B l r HAB Hl Hr IAB Il Ir => 
+      stop
+      dsimp only [denote', Term.denote_ty', Term.denote_ty, 
+        Stlc.HasType.interp, Term.stlc, stlc_ty, term, Term.stlc_ty, 
+        Ty.interp.pair]
+      generalize Hli: Stlc.HasType.interp _ _ = li;
+      have Il' := Hli ▸ Il HΓ G HG;
+      generalize Hri: Stlc.HasType.interp _ _ = ri;
+      have HB: (_::Γ) ⊢ B: type := by cases HAB; assumption;
+      have Ir' := Ir HΓ G HG;
+      --rw [HasType.stlc_ty_subst0] at Ir';
+      cases li with
+      | some li => 
+        cases ri with
+        | some ri => sorry
+        | none => 
+          apply Hr.term_regular.denote_ty_non_null
+          dsimp only [denote'] at Ir'
+          apply Term.denote_ty_transport rfl rfl rfl _ Ir'
+          simp only []
+          rw [<-Stlc.HasType.interp_transport_inner _ _ rfl HB.stlc_ty_subst.symm]
+          exact (interp_eq_none' Hri).symm
+      | none => exact Hl.term_regular.denote_ty_non_null Il'
+    | @let_pair Γ A B C e e' k He HA HB HC He' Ie IA IB IC Ie' =>
+      cases k with
+      | type => sorry
+      | prop => sorry
+    | inj_l He HB Ie IB => 
+      stop
+      dsimp only [
+        denote', Term.denote_ty', Term.denote_ty, Term.stlc, 
+        stlc_ty, Term.stlc_ty, Stlc.HasType.interp,
+        Ty.interp.inl
+      ]
+      generalize Hei: Stlc.HasType.interp _ _ = ei;
+      have Ie' := Hei ▸ Ie HΓ G HG;
+      cases ei with
+      | some ei => 
+        dsimp only [Option.map, Option.bind, Function.comp]
+        exact Ie'
+      | none => exact He.term_regular.denote_ty_non_null Ie'
+    | inj_r He HA Ie IA => 
+      stop
+      dsimp only [
+        denote', Term.denote_ty', Term.denote_ty, Term.stlc, 
+        stlc_ty, Term.stlc_ty, Stlc.HasType.interp,
+        Ty.interp.inl
+      ]
+      generalize Hei: Stlc.HasType.interp _ _ = ei;
+      have Ie' := Hei ▸ Ie HΓ G HG;
+      cases ei with
+      | some ei => 
+        dsimp only [Option.map, Option.bind, Function.comp]
+        exact Ie'
+      | none => exact He.term_regular.denote_ty_non_null Ie'
+    | @case Γ A B C e l r k He HA HB HC Hl Hr Ie IA IB IC Il Ir => 
+      stop
+      cases k with
+      | type => 
+        dsimp only [denote']
+        dsimp only [Term.stlc, Term.stlc_ty, stlc_ty, Stlc.HasType.interp]
+        have HAB: Γ ⊢ Term.coprod A B: type := HasType.coprod HA HB;
+        have Ie' := Ie HΓ G HG;
+        dsimp only [Term.stlc, Term.stlc_ty, stlc_ty, Stlc.HasType.interp] at Ie';
+        generalize Hei: Stlc.HasType.interp (_ : _⊧Term.stlc e _:_) _ = ei;
+        --TODO: wait for Zulip to answer regarding the requirement to have
+        -- Stlc.HasType.interp_irrel here.
+        rw [Stlc.HasType.interp_irrel] at Ie'
+        rw [Hei] at Ie'
+        cases ei with
+        | some e => 
+          cases e with
+          | inl a => 
+            simp only [Ty.interp.case]
+            sorry --TODO: appropriate typecasting for Il
+          | inr b => 
+            simp only [Ty.interp.case]
+            sorry --TODO: appropriate typecasting for Il
+        | none => exact False.elim (HAB.denote_ty_non_null Ie')
+      | prop => 
+        dsimp only [denote']
+        sorry
+    | elem => sorry
+    | let_set => sorry
+    | lam_pr => sorry
+    | app_pr HφA Hl Hr IφA Il Ir => 
+      stop
+      dsimp only [denote', Term.denote_ty, Term.denote_ty']
+      sorry
+    | lam_irrel => sorry
+    | app_irrel => sorry
+    | @repr Γ A B l r HAB Hl Hr IAB Il Ir =>
+      stop 
+      dsimp only [
+        denote', Stlc.HasType.interp, Term.stlc, Term.stlc_ty, stlc_ty,
+        Term.denote_ty', Term.denote_ty
+      ]
+      apply And.intro
+      . sorry -- not_none + Ir?
+      . exists Hl.stlc.interp G.downgrade
+        sorry
+    | let_repr => sorry
+    | abort Hp HA Ip IA => exact False.elim (Ip HΓ G HG)
+    | dconj => sorry
+    | let_conj => sorry
+    | disj_l He HB Ie IB => exact Or.inl (Ie HΓ G HG)
+    | disj_r He HB Ie IB => exact Or.inr (Ie HΓ G HG)
+    | case_pr He HA HB HC Hl Hr Ie IA IB IC Il Ir => 
+      dsimp only [
+        denote', Stlc.HasType.interp, Term.stlc, Term.stlc_ty, stlc_ty,
+        Term.denote_ty', Term.denote_ty
+      ]
+      have Ie' := Ie HΓ G HG;
+      cases Ie' with
+      | inl Ie' => sorry
+      | inr Ie' => sorry
+    | imp => sorry
+    | mp => sorry
+    | general => sorry
+    | inst => sorry
+    | @wit Γ A φ l r HAφ Hl Hr IAφ Il Ir =>
+      stop
+      exists Hl.stlc.interp G
+      --TODO: upgrade theorems for IsCtx and context denotation
+      have Il' := Il sorry (Context.upgrade_idem.symm ▸ G) sorry;
+      apply And.intro
+      . dsimp only [denote', Term.denote_ty'] at Il'
+        sorry
+      . sorry
+    | let_wit => sorry
+    | refl Ha => exact ⟨Ha.stlc, Ha.stlc, rfl⟩
+    | sym HA => exact HA.sym_axiom
+    | trans HA => exact HA.trans_axiom 
+    | cong => 
+      dsimp only [denote', Annot.denote]
+      sorry
+    | beta => 
+      dsimp only [denote', Annot.denote]
+      sorry
+    | @eta Γ A B f Hf HA If IA => 
+      stop
+      have px
+        : Γ.upgrade.stlc ⊧ (Term.eta_ex A B f).stlc Γ.upgrade.sparsity
+          : Ty.arrow A.stlc_ty B.stlc_ty 
+        := sorry;
+      have py
+        : Γ.upgrade.stlc ⊧ f.stlc Γ.upgrade.sparsity
+          : Ty.arrow A.stlc_ty B.stlc_ty 
+        := sorry;
+      --TODO: get rid of double upgrade...
+      have If' := If sorry (Context.upgrade_idem.symm ▸ G) sorry;
+      have HAB := Hf.term_regular;
+      have ⟨yi, Hyi⟩ := HAB.denote_ty_some If';
+      dsimp only [denote'] at If';
+      exists px, py;
+      unfold Term.eta_ex
+      dsimp only [Term.stlc_ty, Stlc.HasType.interp, Term.stlc]
+      simp only []
+      sorry
+    | irir Hf Hx Hy => exact ⟨sorry, sorry, rfl⟩
+    | prir Hf Hx Hy => exact ⟨sorry, sorry, rfl⟩
+    | succ => 
+      intro x H;
+      cases x with
+      | none => cases H
+      | some x => exact True.intro
+    | @natrec Γ C e z s k HC He Hz Hs IC Ie Iz Is => sorry
+    | _ => exact True.intro
+  }
