LogicalRefinement/Denot/Wk.lean
@@ -1,0 +1,45 @@
+import LogicalRefinement.Untyped
+import LogicalRefinement.Typed
+import LogicalRefinement.Stlc
+import LogicalRefinement.Denot.Basic
+
+open AnnotSort
+open Annot
+
+theorem Term.denote_wk1_ty
+  (A: Term) 
+  (B: Term)
+  (Γ: Context)
+  (x: B.stlc_ty.interp) 
+  (G: Γ.upgrade.stlc.interp) 
+  (a: A.stlc_ty.interp)
+  (a': A.wk1.stlc_ty.interp)
+  (Haa': a' = A.stlc_ty_wk1 ▸ a)
+  (H: A.denote_ty' G a) 
+  : @denote_ty' A.wk1 ((Hyp.val B type)::Γ) (x, G) a'
+  := sorry
+  
+theorem Term.denote_wk1_prop
+  (A: Term) 
+  (φ: Term)
+  (Γ: Context)
+  (G: Γ.upgrade.stlc.interp) 
+  (a: A.stlc_ty.interp)
+  (a': A.wk1.stlc_ty.interp)
+  (Haa': a' = A.stlc_ty_wk1 ▸ a)
+  (H: @denote_ty' A Γ G a) 
+  : @denote_ty' A.wk1 ((Hyp.val φ prop)::Γ) G a'
+  := sorry
+  
+theorem Term.denote_wk1_gst
+  (A: Term) 
+  (B: Term)
+  (Γ: Context) 
+  (x: B.stlc_ty.interp)
+  (G: Γ.upgrade.stlc.interp) 
+  (a: A.stlc_ty.interp)
+  (a': A.wk1.stlc_ty.interp)
+  (Haa': a' = A.stlc_ty_wk1 ▸ a)
+  (H: A.denote_ty' G a) 
+  : @denote_ty' A.wk1 ((Hyp.gst B)::Γ) (x, G) a'
+  := sorry
